Cleanup 2

project/algebraic/algebraic_graph.v
@@ -32,20 +32,18 @@ Definition from_nat (n:nat) : AG nat :=
 Coercion from_nat : nat >-> AG.
 
 
+
+
 (* *** has more priority than +++ *)
 Notation "ag1 +++ ag2" := (Overlay ag1 ag2) (at level 60, right associativity).
-Notation "ag1 --> ag2" := (Connect ag1 ag2) (at level 59, right associativity).
+Notation "ag1 *** ag2" := (Connect ag1 ag2) (at level 59, right associativity).
 
 
 
-
-(* The first part of this file is just the code from the paper copied to coq,
-later on (around l.200) it becomes more experimental *)
-
-
+(* Initially functions from the paper *)
 
 Definition edge {A : Type} (a1 a2 : A) : AG A :=
-    Connect (Vertex a1) (Vertex a2).
+    (Vertex a1) *** (Vertex a2).
 
 Definition vertices {A : Type} (l : list A) : AG A :=
     fold_right Overlay Empty (map Vertex l).
@@ -56,16 +54,8 @@ Definition edges {A : Type} (l : list (A * A)) : AG A :=
 Definition clique {A : Type} (l : list A) : AG A :=
     fold_right Connect Empty (map Vertex l).
 
-Compute clique [1; 2; 3; 4].
-
 Definition makeGraph {A : Type} (vs : list A) (es : list (A * A)) : AG A :=
     Overlay (vertices vs) (edges es).
-
-
-
-Check makeGraph [1; 2; 3] [(1, 2); (2, 3)].
-Check 1 *** (2 +++ 3).
-Compute 1 *** (2 +++ 3) +++ 2 *** 3 = clique[1; 2; 3].
 
 
 Definition path {A : Type} (l : list A) : AG A :=
@@ -75,21 +65,15 @@ Definition path {A : Type} (l : list A) : AG A :=
     | _::xs => edges (combine l xs)
     end.
 
-Compute path [1; 2; 3; 4].
-
-
 Definition circuit {A : Type} (l : list A) : AG A :=
     match l with
     | [] => Empty
     | x::_ => path (l ++ [x])
     end.
 
-Compute circuit [1; 2; 3; 4].
   
 Definition star {A : Type} (x : A) (l : list A) : AG A :=
     Connect (Vertex x) (vertices l).
-
-Compute star 1 [2; 3; 4].
 
 
 Fixpoint gmap {A A' : Type} (f : A -> A') (ag : AG A) : AG A' := 
@@ -100,7 +84,6 @@ Fixpoint gmap {A A' : Type} (f : A -> A') (ag : AG A) : AG A' :=
     | Connect ag1 ag2 => Connect (gmap f ag1) (gmap f ag2)
     end.
 
-Compute gmap (fun x => x + 1) (1 *** 2 +++ 3 *** 4).
 
 Definition mergeVertices {A : Type} (f : A -> bool) (v : A) (ag : AG A) : AG A :=
     gmap (fun x => if f x then v else x) ag.
@@ -112,9 +95,6 @@ Fixpoint toList {A : Type} (ag : AG A) : list A :=
     | Overlay ag1 ag2 => toList ag1 ++ toList ag2
     | Connect ag1 ag2 => toList ag1 ++ toList ag2
     end.
-
-Compute toList (1 *** 2 +++ 3 *** 4).
-
 
 Fixpoint gmapVertex {A A' : Type} (f : AG A -> AG A') (ag : AG A) : AG A' :=
     match ag with
@@ -131,13 +111,8 @@ Definition induce {A : Type} (f : A -> bool) (ag : AG A) : AG A :=
                           end) ag.
 
 
-Compute induce (fun x => eqb  x  1) (1 *** 2 +++ 3 *** 4 +++ 1 *** 2).
-
 Definition removeVertex (x : nat) (ag : AG nat) : AG nat :=
     induce (fun y => negb (eqb x y)) ag.
-
-Compute removeVertex 1 (1 *** 2 +++ 3 *** 4 +++ 1 *** 2).
-
 
 
 Definition splitVertex {A : Type} (x : nat) (l : list nat) (ag : AG nat) : AG nat :=
@@ -145,10 +120,6 @@ Definition splitVertex {A : Type} (x : nat) (l : list nat) (ag : AG nat) : AG na
                           | Vertex y => if eqb x y then vertices l else Vertex y
                           | _ => g'
                           end) ag.
-
-
-
-Compute splitVertex 1 [0; 1] (1 *** (2 +++ 3)).
 
 Fixpoint removeEdge (x y : nat) (ag : AG nat) : AG nat :=
     match ag with
@@ -160,10 +131,6 @@ Fixpoint removeEdge (x y : nat) (ag : AG nat) : AG nat :=
     
     
   
-Compute removeEdge 1 2 (1 *** 2 +++ 3 *** 4).
-
-
-
 Fixpoint transpose {A : Type} (ag : AG A) : AG A :=
     match ag with
     | Empty => Empty
@@ -177,139 +144,11 @@ Fixpoint transpose {A : Type} (ag : AG A) : AG A :=
 
 
 
+(* Start defining own functions: *)
 
-
-
-
-
-
-
-
-
-
-
-(* Here, I start deviating from the paper: *)
-
-
-(* These functions assume no overlapping node labels. It thinks that 1 *** 1 has 2 nodes *)
-
-Fixpoint AG_toList {A : Type} (ag : AG A) : list A :=
-    match ag with
-    | Empty => []
-    | Vertex x => [x]
-    | Overlay ag1 ag2 => AG_toList ag1 ++ AG_toList ag2
-    | Connect ag1 ag2 => AG_toList ag1 ++ AG_toList ag2
-    end.
-
-
-Compute AG_toList (1 *** 2 +++ 3 *** 4).
-Compute AG_toList (1 *** 2 +++ 1 *** 2).
-Compute AG_toList (1 *** 1).
-Compute AG_toList (1 +++ 1).
-
-
-
-Fixpoint countNodes {A : Type} (ag : AG A) : nat :=
-    match ag with
-    | Empty => 0
-    | Vertex x => 1
-    | Overlay ag1 ag2 => countNodes ag1 + countNodes ag2
-    | Connect ag1 ag2 => countNodes ag1 + countNodes ag2
-    end.
-
-Fixpoint countEdges {A : Type} (ag : AG A) : nat :=
-    match ag with
-    | Empty => 0
-    | Vertex x => 0
-    | Overlay ag1 ag2 => countEdges ag1 + countEdges ag2
-    | Connect ag1 ag2 => countEdges ag1 + countEdges ag2 + countNodes ag1 * countNodes ag2
-    end.
-
-
-
-
-
-
-
-
-(* This a somewhat analogous to DFS *)
-(* A little magical, since we are using the returned list as a output list as well as a set *)
-Fixpoint searchGraphUnique (ag : AG nat) (s : set nat) : (list nat) :=
-    match ag with
-    | Empty => []
-    | Vertex x => if set_mem eq_nat_dec x s then [] else [x]
-    | Overlay ag1 ag2 => match searchGraphUnique ag1 s with
-                        | ret => ret ++ searchGraphUnique ag2 (set_union eq_nat_dec s ret)
-                        end
-    | Connect ag1 ag2 => match searchGraphUnique ag1 s with
-                        | ret => ret ++ searchGraphUnique ag2 (set_union eq_nat_dec s ret)
-                        end
-    end.
-
-
-Compute searchGraphUnique (1 *** 2 +++ 3 *** 4) [].
-Compute searchGraphUnique (1 *** 2 +++ 1 *** 2) [].
-Compute searchGraphUnique (1 *** 1) [].
-Compute searchGraphUnique (1 +++ 1) [].
-
-Compute searchGraphUnique (1 *** 2 +++ 2 *** 3 +++ 1 *** 3) [].
-
-
-
-
-
-
-
-
-
-
-
-Fixpoint listEqual (l1 l2 : list nat) : bool :=
-  match l1, l2 with
-    | [], [] => true
-    | x :: xs, y :: ys => if eq_nat_dec x y then listEqual xs ys else false
-    | _, _ => false
-  end.
-
-
-Fixpoint filterOutOf (remove from : list nat) : list nat :=
-  match from with
-    | [] => []
-    | x :: xs => if existsb (fun y => x =? y) remove then filterOutOf remove xs else x :: filterOutOf remove xs
-  end.
-
-(* When getting rid of the fuel, the function is alwas gbeing called on a (bigger list (max amount on nodes in the graph) and a samller graph) these should be summable together. No lexographic order business *) 
-Fixpoint canReachFrom_fuled (ag : AG nat) (acc : list nat) (fuel : nat) : list nat :=
-    match fuel with
-        | 0 => acc
-        | S fuel' => match ag with
-                        | Empty => acc
-                        | Vertex x => acc
-                        | Overlay ag1 ag2 => let result := canReachFrom_fuled ag1 acc fuel' in 
-                                                let result' := canReachFrom_fuled ag2 result fuel' in 
-                                                if listEqual acc result' then acc else canReachFrom_fuled ag result' fuel' (*actually, result' is never smaller*)
-
-                        | Connect ag1 ag2 =>   let result := canReachFrom_fuled ag1 acc fuel' in 
-                                                let result' := canReachFrom_fuled ag2 result fuel' in
-                                                let LHS := searchGraphUnique ag1 [] in
-
-                                                let RHS := searchGraphUnique ag2 [] in
-                                                let result'' := if existsb (fun x => (set_mem eq_nat_dec x LHS)) result' then result' ++ filterOutOf result' RHS else result' in  
-                                                if listEqual acc result'' then acc else canReachFrom_fuled ag result'' fuel'
-                        end
-    end.
-
-Compute canReachFrom_fuled (Vertex 1) [1] 10.
-Compute canReachFrom_fuled ((1 *** 2 +++ 3 *** 4) +++ (2 *** 3)) [1] 7.
-Compute canReachFrom_fuled ((3 *** 4) +++ (1 *** 2 +++ 2 *** 3)) [1] 7.
-Compute canReachFrom_fuled ((1 *** 2) +++ (3 *** 4)) [1; 3] 7.
-
-
-
-
-
+(* The set of nodes of the AG *)
 Fixpoint AG_nodeSet (ag : AG nat) : NatSet.t := 
-let leftAndRight := fun (ag1 ag2 : AG nat) => NatSet.union (AG_nodeSet ag1) (AG_nodeSet ag2) in
+    let leftAndRight := fun (ag1 ag2 : AG nat) => NatSet.union (AG_nodeSet ag1) (AG_nodeSet ag2) in
     match ag with
     | Empty => NatSet.empty
     | Vertex x => NatSet.singleton x
@@ -321,95 +160,41 @@ Definition AG_nodeAmount (ag : AG nat) : nat :=
     NatSet.cardinal (AG_nodeSet ag).
 
 
-
+(* filters the provided set out of the list *)
 Definition NatList_filterOutOf (remove : NatSet.t) (from : list nat) : list nat :=
     filter (fun x => negb (NatSet.mem x remove)) from.
 
-    
-
-
-(* Definition NatList_remove_duplicates (l : list nat) : list nat :=
-  fold_left (fun acc next => if existsb (fun y => y =? next) acc then acc else acc ++ [next]) l nil. *)
-  
-
-
-(* Definition NatList_union (l1 l2 : list nat) :=
-    l1 ++ NatList_remove_duplicates (NatList_filterOutOf l1 l2). *)
-
-(* This is pretty promising :) *)
-
-Fixpoint _singleStep (ag : AG nat) (from : NatSet.t) : NatSet.t :=
-let leftAndRight := fun (ag1 ag2 : AG nat) (from : NatSet.t) => NatSet.union (_singleStep ag1 from) (_singleStep ag2 from) in
- match ag with
-        | Empty => NatSet.empty
-        | Vertex x => NatSet.empty
-        | Overlay ag1 ag2 => leftAndRight ag1 ag2 from
-
-        | Connect ag1 ag2 => NatSet.union (leftAndRight ag1 ag2 from) (
-                                let LHS := AG_nodeSet ag1 in
-                                let RHS := AG_nodeSet ag2 in 
-                                if NatSet.is_empty (NatSet.inter LHS from) then NatSet.empty else RHS
-        )
-                  
+(* Computes the set of nodes reachable from the provided set in a single step in the AG *)
+Fixpoint _singleStep (from : NatSet.t) (ag : AG nat) : NatSet.t :=
+    let leftAndRight := fun (ag1 ag2 : AG nat) (from : NatSet.t) => NatSet.union (_singleStep from ag1) (_singleStep from ag2) in
+    match ag with
+    | Empty => NatSet.empty
+    | Vertex x => NatSet.empty
+    | Overlay ag1 ag2 => leftAndRight ag1 ag2 from
+    | Connect ag1 ag2 => NatSet.union (leftAndRight ag1 ag2 from) (
+                            let LHS := AG_nodeSet ag1 in
+                            let RHS := AG_nodeSet ag2 in 
+                            if NatSet.is_empty (NatSet.inter LHS from) then NatSet.empty else RHS)
     end.
 
-Definition _singleStep_caller (ag : AG nat) (from : list nat) : list nat :=
-    NatSet.elements (_singleStep ag (NatSet_fromList from)).
-
-Compute _singleStep_caller (Vertex 1) [1]. 
-Compute _singleStep_caller ((1 *** 2 +++ 3 *** 4) +++ (2 *** 3)) [1].
-Compute _singleStep_caller ((3 *** 4) +++ (1 *** 2 +++ 2 *** 3)) [1].
-Compute _singleStep_caller ((1 *** 2) +++ (3 *** 4)) [1; 3].
-
-
-(* This is not needed, as using it repeatedly is slow *)
-Fixpoint canReachInNorFewerSteps (ag : AG nat) (from : NatSet.t) (n : nat) : list (NatSet.t) :=
-  match n with
-    | 0 => []
-    | S n' => from :: canReachInNorFewerSteps ag (_singleStep ag from) n'
-  end.
-
-Definition canReachInNorFewerSteps_caller (ag : AG nat) (from : list nat) (n : nat) : list (list nat) :=
-    map NatSet.elements (canReachInNorFewerSteps ag (NatSet_fromList from) n).
-
-Compute canReachInNorFewerSteps_caller (Vertex 1) [1] 3.
-(* Notice, that when we have a cycle, the list is infinite *)
-Compute canReachInNorFewerSteps_caller ((1 *** 2 +++ 3 *** 4) +++ (2 *** 3 +++ 4 *** 1)) [1] 6. 
-Compute canReachInNorFewerSteps_caller ((3 *** 4) +++ (1 *** 2 +++ 2 *** 3)) [1] 4.   
-Compute canReachInNorFewerSteps_caller ((1 *** 2) +++ (3 *** 4)) [1; 3] 10.
-
-
-
-Fixpoint _upToNStepsCap (ag : AG nat) (from visited : NatSet.t) (n : nat) : list NatSet.t :=
-  match n with
+(* Computes a list of the set of reachable nodes until it does not grow (kept track by visited).
+Assumes that all of from are in the AG *)
+Fixpoint _upToNStepsCap_rec  (from visited : NatSet.t) (ag : AG nat) (n : nat) : list NatSet.t :=
+    match n with
     | 0 => []
     | S n' => from ::
-            let next := _singleStep ag from in
-            let nextVisited := NatSet.union visited next in 
-            if NatSet.equal visited nextVisited then [] else
-                 _upToNStepsCap ag next nextVisited  n'
-  end.
+                let next := _singleStep from ag in
+                let nextVisited := NatSet.union visited next in 
+                if NatSet.equal visited nextVisited then [] else
+                    _upToNStepsCap_rec  next nextVisited ag n'
+    end.
 
-
-
-Definition _upToNStepsCapCaller (ag : AG nat) (from : NatSet.t) (n : nat) : list NatSet.t :=
+(* Caller for "_upToNStepsCap_rec" *)
+Definition _upToNStepsCap (from : NatSet.t) (ag : AG nat) (n : nat) : list NatSet.t :=
     let trimmedFrom := NatSet.inter from (AG_nodeSet ag) in
-    _upToNStepsCap ag trimmedFrom trimmedFrom (S n).
+    _upToNStepsCap_rec trimmedFrom trimmedFrom ag (S n).
 
-Definition canReachInNStepsListCapped_caller2 (ag : AG nat) (from : list nat) (n : nat) : list (list nat) :=
-    map NatSet.elements (_upToNStepsCapCaller ag (NatSet_fromList from) n).
-
-Compute canReachInNStepsListCapped_caller2 (Vertex 1) [1] 10.
-Compute canReachInNStepsListCapped_caller2 ((1 *** 2 +++ 3 *** 4) +++ (2 *** 3)) [1] 10.
-Compute canReachInNStepsListCapped_caller2 ((3 *** 4) +++ (1 *** 2 +++ 2 *** 3)) [1] 1000.   
-Compute canReachInNStepsListCapped_caller2 ((1 *** 2) +++ (3 *** 4)) [1; 3] 0.
-
-
-Definition AG_BFS (ag : AG nat) (from : list nat) :=
-    fold_right (fun next acc => NatSet.elements next ++ (NatList_filterOutOf next acc)) [] (_upToNStepsCapCaller ag (NatSet_fromList from) (AG_nodeAmount ag)).
-
-Compute AG_BFS (Vertex 1) [1].
-Compute AG_BFS ((1 *** 2 +++ 3 *** 4) +++ (2 *** 3)) [1].
-Compute AG_BFS ((3 *** 4) +++ (1 *** 2 +++ 2 *** 3)) [1].   
-Compute AG_BFS ((1 *** 2) +++ (3 *** 4)) [1; 3].
+(* Combines result of "_upToNStepsCap" to make a real BFS *)
+Definition AG_BFS (from : list nat) (ag : AG nat) :=
+    fold_right (fun next acc => NatSet.elements next ++ (NatList_filterOutOf next acc)) [] (_upToNStepsCap (NatSet_fromList from) ag (AG_nodeAmount ag)).
 
