project/algebraic/algebraic_graph_theory.v
@@ -1,6 +1,8 @@
 Require Import Setoid Morphisms.
 
+
 Require Import MyProject.project.algebraic.algebraic_graph.
+
 Require Import MyProject.project.algebraic.algebraic_graph_to_RG.
 
 Require Import MyProject.project.relational_graph.
@@ -281,7 +283,7 @@ Admitted.
 
 
 Lemma _singleStep_returns_only_nodes : forall (ag : AG nat) (from : NatSet.t),
-    forall x, NatSet.In x (_singleStep ag from) -> (AG_to_RG_unlE ag).(RG_nodes) x.
+    forall x, NatSet.In x (_singleStep from ag) -> (AG_to_RG_unlE ag).(RG_nodes) x.
 Proof.
     intros. induction ag.
     - simpl in H. apply NatSet_In_is_In_elements in H. simpl in H. destruct H.
@@ -304,15 +306,15 @@ Qed.
 
 Lemma _upToNStepsCap_returns_only_nodes : forall (ag : AG nat) (from s: NatSet.t) (n : nat) x y,
     NatSet.Subset from (AG_nodeSet ag) ->
-    In x (_upToNStepsCap ag from s n) -> NatSet.In y x -> (AG_to_RG_unlE ag).(RG_nodes) y.
+    In x (_upToNStepsCap_rec from s ag n) -> NatSet.In y x -> (AG_to_RG_unlE ag).(RG_nodes) y.
 Proof.
     intros. generalize dependent from. generalize dependent s. induction n.
     - intros. simpl in H. contradiction.
     - intros. simpl in H0. destruct H0.
         + subst. apply In_AG_nodeSet_is_In_RG. unfold NatSet.Subset in H. apply H. assumption.
-        + destruct (NatSet.equal s (NatSet.union s (_singleStep ag from))).  
+        + destruct (NatSet.equal s (NatSet.union s (_singleStep from ag))).  
             -- simpl in H0. contradiction.
-            -- specialize (IHn (NatSet.union s (_singleStep ag from))  (_singleStep ag from) ).
+            -- specialize (IHn (NatSet.union s (_singleStep from ag))  (_singleStep from ag)).
                apply IHn.
                ++ unfold NatSet.Subset. intros.
                apply _singleStep_returns_only_nodes in H2. apply In_AG_nodeSet_is_In_RG. assumption.
@@ -323,14 +325,14 @@ Qed.
             
             
 Lemma _upToNStepsCapCaller_returns_only_nodes : forall (ag : AG nat) (from : NatSet.t) (n : nat) x y,
-    In x (_upToNStepsCapCaller ag from n) -> NatSet.In y x -> (AG_to_RG_unlE ag).(RG_nodes) y.
+    In x (_upToNStepsCap from ag n) -> NatSet.In y x -> (AG_to_RG_unlE ag).(RG_nodes) y.
 Proof.
     intros.
     pose proof _upToNStepsCap_returns_only_nodes.
     specialize (H1 ag (NatSet.inter from (AG_nodeSet ag)) (NatSet.inter from (AG_nodeSet ag)) (S n) x).
     apply H1.
     - unfold NatSet.Subset. intros. apply NatSet.inter_spec in H2. destruct H2. assumption.
-    - unfold _upToNStepsCapCaller in H. apply H.
+    - unfold _upToNStepsCap in H. apply H.
     - assumption.
 Qed.
 
@@ -340,7 +342,7 @@ Qed.
 
 
 Theorem AG_BFS_returns_only_nodes : forall (nodes : list nat) (ag : AG nat),
-  forall x, In x (AG_BFS ag nodes) -> (AG_to_RG_unlE ag).(RG_nodes) x. 
+  forall x, In x (AG_BFS nodes ag) -> (AG_to_RG_unlE ag).(RG_nodes) x. 
 Proof.
     intros. unfold AG_BFS in H. apply consolidation_fold_right_preserves_nodes in H.
         destruct H. destruct H.
@@ -400,7 +402,7 @@ Qed.
 
 
 Theorem AG_BFS_no_duplicates : forall (nodes : list nat) (ag : AG nat),
-  NoDup (AG_BFS ag nodes).
+  NoDup (AG_BFS nodes ag).
 Proof.
     intros.
     unfold AG_BFS.
@@ -408,7 +410,7 @@ Proof.
 Qed.
 
 Theorem AG_BFS_path : forall (nodes : list nat) (ag : AG nat) x y,
-  In x nodes -> (In y (AG_BFS ag nodes) <-> RG_existsPath x y (AG_to_RG_unlE ag)).
+  In x nodes -> (In y (AG_BFS nodes ag) <-> RG_existsPath x y (AG_to_RG_unlE ag)).
 Proof.
   intros.
 Admitted.
@@ -450,7 +452,7 @@ Definition Is_Search_ordered {A B : Type} (l passed : list A) (rg : RG A B) : Pr
 
 
 Theorem AG_BFS_search_order : forall (nodes : list nat) (ag : AG nat),
-    Is_Search_ordered (AG_BFS ag nodes) nodes (AG_to_RG_unlE ag).
+    Is_Search_ordered (AG_BFS nodes ag) nodes (AG_to_RG_unlE ag).
 Proof.
 Admitted.
 
